Semantics/Imp/Typed/Equivalence.lean
@@ -1,0 +1,81 @@
+import Semantics.Imp.Untyped.Natural
+import Semantics.Imp.Untyped.Structural
+import Semantics.Imp.Untyped.Denote
+
+namespace Com
+
+theorem Structural.from_natural {x: Config} (h: x ⟹ s): x ⇒* (skip, s) := by
+  induction h with
+  | skip₁ => exact Star.refl
+  | ass₁ => exact Star.single Step.ass₁
+  | cat₁ _ _ _ ihc ihd => exact Star.cat ihc ihd
+  | cond₁ hb _ ih => exact Star.head Step.cond₁ (hb ▸ ih)
+  | cond₂ hb _ ih => exact Star.head Step.cond₁ (hb ▸ ih)
+  | loop₁ _ hb _ _ ihc ihw =>
+    exact Star.head Step.loop₁ $ Star.trans (hb ▸ Star.cat ihc ihw) Star.refl
+  | loop₂ hb =>
+    exact Star.head Step.loop₁ $ hb ▸ Star.refl
+
+lemma Natural.from_structural_step (h₁: x ⇒ y) (h₂: y ⟹ s): x ⟹ s := by
+  induction h₁ generalizing s with
+  | ass₁ => exact (skip_iff.mp h₂) ▸ Step.ass₁
+  | cat₁ => exact Step.cat₁ _ Step.skip₁ h₂
+  | cat₂ _ ih =>
+    cases h₂ with
+    | cat₁ w hc hd => exact Step.cat₁ w (ih hc) hd
+  | cond₁ => rw [cond_iff']; exact h₂
+  | loop₁ => rw [loop_unfold, cond_iff']; exact h₂
+
+theorem Natural.from_structural (h: x ⇒* (skip, t)): x ⟹ t := by
+  induction h using Structural.Star.head_induction_on with
+  | refl => exact Step.skip₁
+  | head h _ ht => exact from_structural_step h ht
+
+theorem structural_iff_natural: x ⇒* (skip, t) ↔ x ⟹ t := ⟨Natural.from_structural, Structural.from_natural⟩
+
+theorem denote.from_natural {x: Config} (h: x ⟹ t): (x.2, t) ∈ ⟦x.1⟧ := by
+  induction h with
+  | skip₁ => exact SRel.mem_id.mpr rfl
+  | ass₁  => exact SRel.mem_id.mpr rfl
+  | cat₁ t _ _ ih₁ ih₂ => exact ⟨t, ⟨ih₁, ih₂⟩⟩
+  | cond₁ hb _ ih => exact Or.inl ⟨ih, hb⟩
+  | cond₂ hb _ ih => exact Or.inr ⟨ih, hb⟩
+  | loop₁ t hb _ _ ih₁ ih₂ => exact loop_unfold ▸ Or.inl ⟨⟨t, ⟨ih₁, ih₂⟩⟩, hb⟩
+  | loop₂ hb => exact loop_unfold ▸ Or.inr ⟨rfl, hb⟩
+
+theorem Natural.from_denote (h: (s, t) ∈ ⟦c⟧): (c, s) ⟹ t := by
+  revert h
+  induction c generalizing s t with
+  | skip => intro h; cases h; exact Step.skip₁
+  | ass => intro h; simp [denote] at h; exact h ▸ Step.ass₁
+  | cat _ _ ih₁ ih₂ =>
+    intro h
+    cases h with | intro w h =>
+      exact Step.cat₁ w (ih₁ h.left) (ih₂ h.right)
+  | cond _ _ _ ih₁ ih₂ =>
+    intro h
+    cases h with
+    | inl h =>
+      cases h with | intro h hb =>
+        exact Step.cond₁ hb (ih₁ h)
+    | inr h =>
+      cases h with | intro h hb =>
+        exact Step.cond₂ hb (ih₂ h)
+  | loop b c ih =>
+    suffices ⟦loop b c⟧ ⊆ {s | (loop b c, s.1) ⟹ s.2} by apply this
+    apply OrderHom.lfp_le
+    intro ss h
+    cases ss with | mk =>
+      cases h with
+      | inl h =>
+        cases h with | intro h hb =>
+          cases h with | intro w h =>
+            exact Step.loop₁ w hb (ih h.left) h.right
+      | inr h =>
+        cases h with | intro hq hb =>
+          simp at hq
+          exact hq ▸ Step.loop₂ hb
+
+theorem natural_iff_denote: (s, t) ∈ ⟦c⟧ ↔ (c, s) ⟹ t := ⟨Natural.from_denote, denote.from_natural⟩
+
+end Com
