Semantics/Imp/Typed/Syntax.lean
@@ -1,0 +1,96 @@
+import Semantics.State
+import Std.Data.Rat.Basic
+
+@[reducible]
+inductive Val where
+  | int : Int → Val
+  | nat : Nat → Val
+
+inductive Aexp where
+  | val : Val → Aexp
+  | loc : String → Aexp
+  | add : Aexp → Aexp → Aexp
+  | sub : Aexp → Aexp → Aexp
+  | mul : Aexp → Aexp → Aexp
+
+inductive Bexp where
+  | tt
+  | ff
+  | not : Bexp → Bexp
+  | and : Bexp → Bexp → Bexp
+  | or  : Bexp → Bexp → Bexp
+  | eq  : Aexp → Aexp → Bexp
+  | le  : Aexp → Aexp → Bexp
+
+inductive Com where
+  | skip
+  | cat   : Com → Com → Com
+  | ass   : String → Aexp → Com
+  | cond  : Bexp → Com → Com → Com
+  | loop  : Bexp → Com → Com
+
+def Config := Com × State
+
+-- Meta syntax
+notation:50 x:50 ";;" e:51 => Com.cat x e
+
+-- Syntax of the language
+declare_syntax_cat imp
+
+-- general
+syntax "(" imp ")" : imp
+-- imp
+syntax num : imp
+syntax "[" num "]" : imp
+syntax ident: imp
+syntax:60 imp:60 "+" imp:61 : imp
+syntax:60 imp:60 "-" imp:61 : imp
+syntax:70 imp:70 "*" imp:71 : imp
+-- bexp
+syntax:80 "!" imp:81 : imp
+syntax:70 imp:70 "==" imp:71 : imp
+syntax:70 imp:70 "<=" imp:71 : imp
+syntax:65 imp:65 "||" imp:66 : imp
+syntax:65 imp:65 "&&" imp:66 : imp
+-- stmt
+syntax:50 imp:50 "=" imp:51 : imp
+syntax:40 imp:40 ";" imp:41 : imp
+syntax "if" imp "{" imp "}" "else" "{" imp "}" : imp
+syntax "while" imp "{" imp "}" : imp
+
+-- meta
+syntax "⦃" imp "⦄" : term
+
+macro_rules
+  -- keywords
+  | `(⦃skip⦄) => `(Com.skip)
+  | `(⦃true⦄)   => `(Bexp.tt)
+  | `(⦃false⦄)   => `(Bexp.ff)
+  -- general
+  | `(⦃($x)⦄) => `(⦃$x⦄)
+  -- imp
+  | `(⦃$x:ident⦄) => `(Aexp.loc $(Lean.quote (toString x.getId)))
+  | `(⦃$n:num⦄) => `(Aexp.val (Val.int $n))
+  | `(⦃[$n:num]⦄) => `(Aexp.val (Val.nat $n))
+  | `(⦃$x + $y⦄)  => `(Aexp.add ⦃$x⦄ ⦃$y⦄)
+  | `(⦃$x - $y⦄)  => `(Aexp.sub ⦃$x⦄ ⦃$y⦄)
+  | `(⦃$x * $y⦄)  => `(Aexp.mul ⦃$x⦄ ⦃$y⦄)
+  -- bexp
+  | `(⦃!$x⦄)      => `(Bexp.not ⦃$x⦄)
+  | `(⦃$x == $y⦄)  => `(Bexp.eq ⦃$x⦄ ⦃$y⦄)
+  | `(⦃$x <= $y⦄)  => `(Bexp.le ⦃$x⦄ ⦃$y⦄)
+  | `(⦃$x && $y⦄)  => `(Bexp.and ⦃$x⦄ ⦃$y⦄)
+  | `(⦃$x || $y⦄)  => `(Bexp.or ⦃$x⦄ ⦃$y⦄)
+  -- stmt
+  | `(⦃$x:ident = $y⦄) => `(Com.ass $(Lean.quote (toString x.getId)) ⦃$y⦄)
+  | `(⦃$x ; $y⦄)       => `(Com.cat ⦃$x⦄ ⦃$y⦄)
+  | `(⦃if $b {$x} else {$y}⦄) => `(Com.cond ⦃$b⦄ ⦃$x⦄ ⦃$y⦄)
+  | `(⦃while $b {$x}⦄) => `(Com.loop ⦃$b⦄ ⦃$x⦄)
+
+#check ⦃z = 4; if 3 <= 2 {y = 4 + 2} else {skip}⦄
+#check ⦃while true {skip}⦄
+#check ⦃skip⦄
+#check ⦃x = 5⦄
+#check ⦃x = 5; y = [6]⦄
+#check ⦃if x == 5 {y = 6} else {z = 7}⦄
+#check ⦃x = 0; while !(x == 5) {skip; skip; x = x + 1}⦄
