Semantics/Imp/Untyped/Aexp.lean
@@ -1,0 +1,118 @@
+import Semantics.Imp.Untyped.Syntax
+import Semantics.Relation
+
+namespace Aexp
+namespace Natural
+
+-- Operational semantics of aexp
+inductive Step: Aexp × State → Val → Prop
+  | val₁:
+    Step (val n, _) n
+
+  | loc₁:
+    Step (loc x, s) (s x)
+
+  | add₁ (h₁: Step (a, s) n) (h₂: Step (b, s) m):
+    Step (add a b, s) (n + m)
+
+  | sub₁ (h₁: Step (a, s) n) (h₂: Step (b, s) m):
+    Step (sub a b, s) (n - m)
+
+  | mul₁ (h₁: Step (a, s) n) (h₂: Step (b, s) m):
+    Step (mul a b, s) (n * m)
+
+infix:110 " ⟹ " => Step
+
+theorem reducing: reducing Step := by {
+  unfold reducing
+  intro t
+  cases t with | mk f s => {
+    induction f with
+    | val n => exact ⟨n, Step.val₁⟩
+    | loc x => exact ⟨s x, Step.loc₁⟩
+    | add a b ih₁ ih₂ =>
+      cases ih₁ with | intro w₁ ih₁ =>
+        cases ih₂ with | intro w₂ ih₂ =>
+          exact ⟨w₁ + w₂, Step.add₁ ih₁ ih₂⟩
+    | sub a b ih₁ ih₂ =>
+      cases ih₁ with | intro w₁ ih₁ =>
+        cases ih₂ with | intro w₂ ih₂ =>
+          exact ⟨w₁ - w₂, Step.sub₁ ih₁ ih₂⟩
+    | mul a b ih₁ ih₂ =>
+      cases ih₁ with | intro w₁ ih₁ =>
+        cases ih₂ with | intro w₂ ih₂ =>
+          exact ⟨w₁ * w₂, Step.mul₁ ih₁ ih₂⟩
+  }
+}
+
+theorem determinist: determinist Step := by {
+  unfold determinist
+  intro a b c h₁ h₂
+  induction h₁ generalizing c with
+  | val₁ => cases h₂; rfl
+  | loc₁ => cases h₂; rfl
+  | add₁ _ _ ih₁ ih₂ =>
+    cases h₂ with | add₁ h₁ h₂ =>
+      exact (ih₁ _ h₁) ▸ (ih₂ _ h₂) ▸ rfl
+  | sub₁ _ _ ih₁ ih₂ =>
+    cases h₂ with | sub₁ h₁ h₂ =>
+      exact (ih₁ _ h₁) ▸ (ih₂ _ h₂) ▸ rfl
+  | mul₁ _ _ ih₁ ih₂ =>
+    cases h₂ with | mul₁ h₁ h₂ =>
+      exact (ih₁ _ h₁) ▸ (ih₂ _ h₂) ▸ rfl
+}
+
+end Natural
+
+-- Denotational semantics of arithmetic expressions
+@[reducible]
+def reduce (a: Aexp) (s: State): Val :=
+  match a with
+  | val n => n
+  | loc x => s x
+  | add a b => reduce a s + reduce b s
+  | sub a b => reduce a s - reduce b s
+  | mul a b => reduce a s * reduce b s
+
+infix:110 "⇓" => reduce
+
+-- relational definition is equal to recursive
+theorem reduce.from_natural (h: as ⟹ n): reduce.uncurry as = n :=
+  by induction h with
+  | val₁ => rfl
+  | loc₁ => rfl
+  | _ _ _ ih₁ ih₂ => exact ih₁ ▸ ih₂ ▸ rfl
+
+theorem Natural.from_reduce {a: Aexp} (h: a⇓s = n): (a,s) ⟹ n :=
+  by induction a generalizing n with
+  | val _ => exact h ▸ Step.val₁
+  | loc _ => exact h ▸ Step.loc₁
+  | add _ _ l r => exact h ▸ Step.add₁ (l rfl) (r rfl)
+  | sub _ _ l r => exact h ▸ Step.sub₁ (l rfl) (r rfl)
+  | mul _ _ l r => exact h ▸ Step.mul₁ (l rfl) (r rfl)
+
+@[simp] theorem Step_iff_reduce: (a, s) ⟹ n ↔ a⇓s = n := ⟨reduce.from_natural, Natural.from_reduce⟩
+@[simp] theorem Step_iff_reduce': (a, s) ⟹ (a⇓s) := Natural.from_reduce rfl
+
+protected instance Step.equiv: Setoid Aexp where
+  r a b := ∀ s n, (a, s) ⟹ n = (b, s) ⟹ n
+  iseqv := {
+    refl := λ _ _ _ ↦ Eq.refl _
+    symm := λ h s n ↦ Eq.symm (h s n)
+    trans := λ h₁ h₂ x n ↦ (h₁ x n) ▸ (h₂ x n)
+  }
+
+instance reduce.equiv: Setoid Aexp where
+  r a b := ∀s, a⇓s = b⇓s
+  iseqv := ⟨λ _ _ ↦ Eq.refl _, (Eq.symm $ · ·) , λ h₁ h₂ s ↦ (h₁ s) ▸ (h₂ s)⟩
+
+protected theorem Step_eq_eq_reduce_eq: Step.equiv.r a b ↔ reduce.equiv.r a b := by
+  constructor <;> intro h
+  . simp [Setoid.r] at *
+    intro s
+    specialize h s
+    exact h
+  . simp [Setoid.r] at *
+    simp [h]
+
+end Aexp
