Semantics/Imp/Untyped/Bexp.lean
@@ -1,0 +1,92 @@
+import Semantics.Imp.Untyped.Aexp
+
+namespace Bexp
+namespace Natural
+
+-- Operational semantics of Bexp
+inductive Step: Bexp × State → Bool → Prop
+  | tt₁:
+    Step (tt, _) true
+
+  | ff₁:
+    Step (ff, _) false
+
+  | eq₁:
+    Step (eq a b, s) (a⇓s = b⇓s)
+
+  | le₁:
+    Step (le a b, s) (a⇓s ≤ b⇓s)
+
+  | not₁ {a: Bexp} (h: Step (a,s) n):
+    Step (not a, s) (!n)
+
+  | and₁ {a b: Bexp} (h₁: Step (a,s) n) (h₂: Step (b,s) m):
+    Step (and a b, s) (n && m)
+
+  | or₁ {a b: Bexp} (h₁: Step (a,s) n) (h₂: Step (b,s) m):
+    Step (or a b, s) (n || m)
+
+infix:110 " ⟹ " => Step
+
+end Natural
+
+-- Denotational semantics of Bexp
+@[reducible, simp] def reduce (b: Bexp) (s: State): Bool :=
+  match b with
+  | tt      => true
+  | ff      => false
+  | not b   => !reduce b s
+  | and a b => reduce a s && reduce b s
+  | or a b  => reduce a s || reduce b s
+  | eq a b  => a⇓s = b⇓s
+  | le a b  => a⇓s ≤ b⇓s
+
+infix:110 "⇓" => reduce
+
+-- relational definition is equivalent to recursive
+theorem Natural.from_reduce {b: Bexp} (h: b⇓s = x): (b, s) ⟹ x :=
+  by induction b generalizing x with
+  | tt => exact h ▸ Step.tt₁
+  | ff => exact h ▸ Step.ff₁
+  | eq => exact h ▸ Step.eq₁
+  | le => exact h ▸ Step.le₁
+  | not _ ih => exact h ▸ Step.not₁ (ih rfl)
+  | and _ _ l r => exact h ▸ Step.and₁ (l rfl) (r rfl)
+  | or _ _  l r => exact h ▸ Step.or₁  (l rfl) (r rfl)
+
+theorem reduce.from_natural {bs: Bexp × State} (h: bs ⟹ x): reduce.uncurry bs = x :=
+  by induction h with
+  | tt₁ => rfl
+  | ff₁ => rfl
+  | eq₁ => rfl
+  | le₁ => rfl
+  | not₁ _ ih => exact ih ▸ rfl
+  | _ _ _ ih₁ ih₂ => exact ih₁ ▸ ih₂ ▸ rfl
+
+@[simp] theorem Step_eq_reduce {b: Bexp}: (b,s) ⟹ r ↔ b⇓s = r := ⟨reduce.from_natural, Natural.from_reduce⟩
+
+theorem not_true_eq_false: (!b⇓s) = (not b)⇓s := by simp
+
+protected instance Step.equiv: Setoid Bexp where
+  r a b := ∀ s n, (a, s) ⟹ n = (b, s) ⟹ n
+  iseqv := {
+    refl := λ _ _ _ ↦ Eq.refl _
+    symm := λ h s n ↦ Eq.symm (h s n)
+    trans := λ h₁ h₂ x n ↦ (h₁ x n) ▸ (h₂ x n)
+  }
+
+@[reducible, simp]
+instance reduce.equiv: Setoid Bexp where
+  r a b:= ∀s, a⇓s = b⇓s
+  iseqv := ⟨λ _ _ ↦ Eq.refl _, (Eq.symm $ · ·) , λ h₁ h₂ s ↦ (h₁ s) ▸ (h₂ s)⟩
+
+protected theorem Step_eq_eq_reduce_eq: Step.equiv.r a b ↔ reduce.equiv.r a b := by
+  constructor <;> intro h
+  . simp [Setoid.r] at *
+    intro s
+    specialize h s
+    exact h
+  . simp [Setoid.r] at *
+    simp [h]
+
+end Bexp
