Semantics/Imp/Untyped/Denote.lean
@@ -1,0 +1,100 @@
+import Semantics.Imp.Untyped.Bexp
+
+import Mathlib.Data.Set.Basic
+import Mathlib.Order.CompleteLattice
+import Mathlib.Data.Set.Lattice
+import Mathlib.Order.FixedPoints
+
+namespace SRel
+
+/-!
+## Set relation `Set (α × β)`, aka graph of partial function, aka Lana Del Rey
+-/
+
+notation:20 α " →ᵍ " β => Set (α × β)
+
+def id: α →ᵍ α := {p | p.1 = p.2}
+
+@[simp] theorem mem_id {a b: α}:
+  (a, b) ∈ @id α ↔ a = b := Iff.rfl
+
+def comp (f g: α →ᵍ α): α →ᵍ α :=
+  {x | ∃z, (x.1, z) ∈ f ∧ (z, x.2) ∈ g}
+
+infixl:90 " ○ " => SRel.comp
+
+@[simp] theorem mem_comp {f g: α →ᵍ α}:
+  x ∈ f ○ g ↔ ∃z, (x.1, z) ∈ f ∧ (z, x.2) ∈ g := Iff.rfl
+
+@[reducible]
+def restrict (s: Set α) (f: α →ᵍ β): α →ᵍ β :=
+  {x ∈ f | x.1 ∈ s}
+
+theorem monotone_comp [PartialOrder α] {f g: α → (β →ᵍ β)}
+  (hf: Monotone f) (hg: Monotone g):
+  Monotone λ x ↦ f x ○ g x :=
+  λ _ _ h _ ⟨z, h₁, h₂⟩ ↦ ⟨z, hf h h₁, hg h h₂⟩
+
+theorem monotone_restrict [PartialOrder α] {f : α → (β →ᵍ β)} {s: Set β}
+  (hf: Monotone f):
+  Monotone (restrict s $ f ·) :=
+  λ _ _ h _ ⟨z, h₁⟩ ↦ ⟨hf h z, h₁⟩
+
+end SRel
+
+namespace Com
+
+def denote_loop (b: Bexp) (f: State →ᵍ State): (State →ᵍ State) →o (State →ᵍ State) :=
+  ⟨λ g ↦ (SRel.restrict {s | b⇓s = true} $ f ○ g) ∪ (SRel.restrict {s | b⇓s = false} SRel.id),
+    Monotone.union
+      (SRel.monotone_restrict (SRel.monotone_comp monotone_const monotone_id))
+      (SRel.monotone_restrict monotone_const)⟩
+
+def denote: Com → (State →ᵍ State)
+  | skip       => SRel.id
+  | ass x a    => {s | s.2 = s.1⟪x ≔ a⇓s.1⟫}
+  | c;;d       => c.denote ○ d.denote
+  | cond b c d => (SRel.restrict {s | b⇓s = true} c.denote) ∪ (SRel.restrict {s | b⇓s = false} d.denote)
+  | loop b c   => OrderHom.lfp (denote_loop b c.denote)
+
+notation (priority := high) "⟦" c "⟧" => denote c
+
+#simp [denote] (⟪⟫, ⟪⟫⟪"x"≔5⟫⟪"x"≔1⟫) ∈ ⟦⦃x = 5; if x == 1 {skip} else {x = 1}⦄⟧
+#simp [denote] (⟪⟫, ⟪⟫⟪"x"≔5⟫) ∈ ⟦⦃x = 5; while x == 1 {x = 1}⦄⟧
+
+namespace denote
+
+@[simp]
+instance equiv: Setoid Com := ⟨(⟦·⟧ = ⟦·⟧), ⟨(refl ⟦.⟧), symm, Eq.trans⟩⟩
+
+theorem skipl: (skip;;c) ≈ c := by
+  simp [HasEquiv.Equiv, denote, SRel.comp]
+
+theorem skipr: (c;;skip) ≈ c := by
+  simp [HasEquiv.Equiv, denote, SRel.comp]
+
+theorem loop_unfold: loop b c ≈ cond b (c;;loop b c) skip := by
+  simp [HasEquiv.Equiv]
+  exact Eq.symm $ OrderHom.map_lfp $ denote_loop b ⟦c⟧
+
+/-
+## Congruence
+-/
+
+theorem cat_congr (hc: c₁ ≈ c₂) (hd: d₁ ≈ d₂):
+  (c₁;;d₁) ≈ (c₂;;d₂) := by
+  simp [HasEquiv.Equiv, denote]
+  exact hc ▸ hd ▸ rfl
+
+theorem cond_congr (hc: c₁ ≈ c₂) (hd: d₁ ≈ d₂):
+  (cond b c₁ d₁) ≈ (cond b c₂ d₂) := by
+  simp [HasEquiv.Equiv, denote]
+  exact hc ▸ hd ▸ rfl
+
+theorem loop_congr (hc: c₁ ≈ c₂):
+  (loop b c₁) ≈ (loop b c₂) := by
+  simp [HasEquiv.Equiv, denote]
+  exact hc ▸ rfl
+
+end denote
+end Com
