Semantics/Imp/Untyped/Natural.lean
@@ -1,0 +1,176 @@
+import Semantics.Imp.Untyped.Bexp
+
+namespace Com
+namespace Natural
+
+inductive Step: Config → State → Prop
+  | skip₁:
+    Step (skip, s) s
+
+  | ass₁:
+    Step (ass x a, s) (s⟪x ≔ a⇓s⟫)
+
+  | cat₁ t
+    (hc: Step (c, s) t) (hd: Step (d, t) u):
+    Step (c;;d, s) u
+
+  | cond₁ {b: Bexp}
+    (hb: b⇓s = true) (hc: Step (c, s) t):
+    Step (cond b c d, s) t
+
+  | cond₂ {b: Bexp}
+    (hb: b⇓s = false) (hd: Step (d, s) t):
+    Step (cond b c d, s) t
+
+  | loop₁ {b: Bexp} u
+    (hb: b⇓s = true) (hc: Step (c, s) u) (hw: Step (loop b c, u) t):
+    Step (loop b c, s) t
+
+  | loop₂ {b: Bexp}
+    (hb: b⇓s = false):
+    Step (loop b c, s) s
+
+infix:110 " ⟹ " => Step
+
+theorem demo₁: (⦃x = 5⦄, ⟪⟫) ⟹ ⟪⟫⟪"x"≔5⟫ := Step.ass₁
+
+theorem demo₂:
+  (⦃x = 2; if x <= 1 {y = 3} else {z = 4}⦄, ⟪⟫) ⟹
+  (⟪⟫⟪"x"≔2⟫⟪"z"≔4⟫) := Step.cat₁ _ Step.ass₁ $ Step.cond₂ rfl Step.ass₁
+
+/-
+## Rewriting rules
+-/
+
+theorem skip_iff: (skip, s) ⟹ t ↔ s = t := by
+  apply Iff.intro <;> intro h
+  . cases h; rfl
+  . exact h ▸ Step.skip₁
+
+theorem cat_iff: (c;;d, s) ⟹ t ↔ ∃ w, (c, s) ⟹ w ∧ (d, w) ⟹ t := by
+  apply Iff.intro <;> intro h
+  . cases h with | cat₁ t h₁ h₂ =>
+      exact ⟨t, ⟨h₁, h₂⟩⟩
+  . cases h with | intro w h =>
+      exact Step.cat₁ w h.1 h.2
+
+theorem cond_iff: (cond b c d, s) ⟹ t ↔ bif b⇓s then (c, s) ⟹ t else (d, s) ⟹ t := by
+  constructor <;> intro h
+  . cases h with
+    | cond₁ hb hc => exact hb ▸ hc
+    | cond₂ hb hc => exact hb ▸ hc
+  . cases hb: b⇓s with
+    | true => exact Step.cond₁ hb $ (cond_true ((c, s) ⟹ t) _) ▸ hb ▸ h
+    | false => exact Step.cond₂ hb $ (cond_false _ ((d, s) ⟹ t)) ▸ hb ▸ h
+
+theorem cond_iff': (cond b c d, s) ⟹ t ↔ (bif b⇓s then c else d, s) ⟹ t := by
+  rw [cond_iff]; cases b⇓s <;> simp
+
+theorem loop_iff: (loop b c, s) ⟹ t ↔
+  (bif b⇓s then ∃ w, (c, s) ⟹ w ∧ (loop b c, w) ⟹ t else s = t) := by
+  apply Iff.intro <;> intro h
+  . cases h with
+    | loop₁ t hb hc hw =>
+      exact hb ▸ ⟨t, ⟨hc, hw⟩⟩
+    | loop₂ hb =>
+      exact hb ▸ rfl
+  . cases hb: b⇓s with
+    | true =>
+      rw [hb] at h
+      cases h with | intro w h =>
+        exact Step.loop₁ w hb h.1 h.2
+    | false =>
+      exact (hb ▸ h) ▸ Step.loop₂ hb
+
+/-
+## Behavioral equivalence
+-/
+
+instance equiv: Setoid Com where
+  r c d := ∀ s t, (c, s) ⟹ t ↔ (d, s) ⟹ t
+  iseqv := {
+    refl := λ _ _ _ ↦ Iff.refl _
+    symm := (Iff.symm $ · · ·)
+    trans := λ h₁ h₂ x n ↦ Iff.trans (h₁ x n) (h₂ x n)
+  }
+
+theorem skipl: (skip;;c) ≈ c := by
+  intro _ _
+  constructor
+  . intro h; cases h with | cat₁ _ hc hd =>
+      exact skip_iff.mp hc ▸ hd
+  . exact (Step.cat₁ _ Step.skip₁ ·)
+
+theorem skipr: (c;;skip) ≈ c := by
+  intro _ _
+  constructor
+  . intro h; cases h with | cat₁ _ hc hd =>
+      exact skip_iff.mp hd ▸ hc
+  . exact (Step.cat₁ _ · Step.skip₁)
+
+theorem cond_true (h: b ≈ Bexp.tt): cond b c d ≈ c := by
+  intro _ _
+  rw [cond_iff, h]
+  rfl
+
+theorem cond_false (h: b ≈ Bexp.ff): cond b c d ≈ d := by
+  intro _ _
+  rw [cond_iff, h]
+  exact Iff.rfl
+
+theorem loop_unfold:
+  loop b c ≈ cond b (c;;loop b c) skip := by
+  intro s t
+  constructor <;> intro h
+  . rw [cond_iff]
+    cases h with
+    | loop₁ w hb hc hw => exact hb ▸ Step.cat₁ w hc hw
+    | loop₂ hb => exact hb ▸ Step.skip₁
+  . rw [loop_iff]
+    rw [cond_iff] at h
+    cases hb: b⇓s <;> rw [hb] at h
+    . exact skip_iff.mp h
+    . exact cat_iff.mp h
+
+/-
+## No normalization
+-/
+
+theorem loop_tt (hq: b ≈ Bexp.tt):
+  ¬((loop b c, s) ⟹ t) := by
+  intro h₁
+  generalize h₂: (loop b c, s) = ww at h₁
+  induction h₁ generalizing s with
+  | loop₁ _ _ _ _ _ ih₂ => cases h₂; apply ih₂; rfl
+  | loop₂ hb => cases h₂; rw [hq] at hb; contradiction
+  | _ => cases h₂
+
+/-
+## Determinism
+-/
+
+theorem determinist {cs: Config} (h₁: cs ⟹ s) (h₂: cs ⟹ t): s = t :=
+  by induction h₁ generalizing t with
+  | cat₁ _ _ _ ih₁ ih₂ => cases h₂ with
+    | cat₁ _ hc hd => exact ih₂ (ih₁ hc ▸ hd)
+
+  | cond₁ hb _ ih => cases h₂ with
+    | cond₁ _ hd => exact ih hd
+    | cond₂ hb₁ hd => simp [hb] at hb₁
+
+  | cond₂ hb _ ih => cases h₂ with
+    | cond₁ hb₁ hd => simp [hb] at hb₁
+    | cond₂ _ hd   => exact ih hd
+
+  | loop₁ _ hb _ _ ih₁ ih₂ => cases h₂ with
+    | loop₁ _ _ hc hw => exact ih₂ (ih₁ hc ▸ hw)
+    | loop₂ hb₁ => simp [hb] at hb₁
+
+  | loop₂ hb => cases h₂ with
+    | loop₁ _ hb₁ => simp [hb] at hb₁
+    | loop₂ => rfl
+
+  | _ => cases h₂; rfl
+
+end Natural
+end Com
