Semantics/Imp/Untyped/Structural.lean
@@ -1,0 +1,87 @@
+import Semantics.Imp.Untyped.Bexp
+
+import Mathlib.Logic.Relation
+
+namespace Com
+namespace Structural
+
+@[reducible]
+inductive Step: Config → Config → Prop where
+  | ass₁:
+    Step (ass x a, s) (skip, s⟪x ≔ a⇓s⟫)
+
+  | cat₁:
+    Step (skip;;c, s) (c, s)
+
+  | cat₂ (h: Step (c, s) (e, t)):
+    Step (c;;d, s) (e;;d, t)
+
+  | cond₁:
+    Step (cond b c d, s) (bif b⇓s then c else d, s)
+
+  | loop₁:
+    Step (loop b c, s) (bif b⇓s then c;;loop b c else skip, s)
+
+infix:110 " ⇒ " => Step
+
+theorem Step.demo₁:
+  (⦃x = 2; while 0 <= x {x = x - 1}⦄, ⟪⟫) ⇒
+      (⦃skip; while 0 <= x {x = x - 1}⦄, ⟪⟫⟪"x"≔2⟫) := cat₂ ass₁
+
+@[simp] theorem Step.cat_iff:
+  (c₁;;c₂, s) ⇒ et ↔
+  (∃e t, (c₁, s) ⇒ (e, t) ∧ et = (e;;c₂, t))
+  ∨ (c₁ = skip ∧ et = (c₂, s)) := by
+  constructor <;> intro h
+  . cases h with
+    | cat₁ => exact Or.inr ⟨rfl, rfl⟩
+    | cat₂ h => exact Or.inl ⟨_, ⟨_, ⟨h, rfl⟩⟩⟩
+  . cases h with
+    | inl h =>
+      cases h with | intro e h =>
+        cases h with | intro t h =>
+          exact h.right ▸ Step.cat₂ h.1
+    | inr h =>
+      cases h with | intro h₁ h₂ =>
+        exact h₁ ▸ h₂ ▸ Step.cat₁
+
+@[simp] lemma Step.cond_iff:
+  (cond b c d, s) ⇒ ss ↔
+  (b⇓s ∧ ss = (c, s)) ∨ (b⇓s = false ∧ ss = (d, s)) := by
+  constructor <;> intro h
+  . cases hb: b⇓s <;> cases h
+    . exact Or.inr ⟨rfl, hb ▸ rfl⟩
+    . exact Or.inl ⟨rfl, hb ▸ rfl⟩
+  . have hss: ss = (bif b⇓s then c else d, s) := by
+      cases hb: b⇓s <;> rw [hb] at h <;> simp at * <;> assumption
+    exact hss ▸ Step.cond₁
+
+@[simp] lemma Step.cond_false {b: Bexp} (hb: b⇓s = false):
+  (cond b c d, s) ⇒ ss ↔ (ss = (d, s)) :=
+  by rw [cond_iff, hb]; simp
+
+infix:110 " ⇒* " => Star Step
+
+theorem StarStep.demo₂:
+  (⦃x = 2; while 0 <= x {x = x - 1}⦄, ⟪⟫) ⇒*
+      (⦃while 0 <= x {x = x - 1}⦄, ⟪⟫⟪"x"≔2⟫) :=
+  Star.head (Step.cat₂ Step.ass₁) (Star.head Step.cat₁ Star.refl)
+
+theorem StarStep.cat_skip_cat
+  (h: (c, s) ⇒* (skip, t)):
+  (c;;d, s) ⇒* (skip;;d, t) :=
+  Star.lift (λ (x: Config) ↦ (x.1;;d, x.2)) (λ _ _ h => Step.cat₂ h) h
+
+theorem StarStep.cat
+  (h₁: (c₁, s) ⇒* (skip, s₁))
+  (h₂: (c₂, s₁) ⇒* (skip, s₂)):
+  (c₁;;c₂, s) ⇒* (skip, s₂) :=
+  Star.trans (cat_skip_cat h₁) (Star.trans (Star.single Step.cat₁) h₂)
+
+theorem StarStep.cat_no_influence
+  (h: (c₁, s) ⇒* (skip, s₁)):
+  (c₁;;c₂, s) ⇒* (c₂, s₁) :=
+  Star.trans (cat_skip_cat h) (Star.single Step.cat₁)
+
+end Structural
+end Com
