Semantics/Stlc/Natural.lean
@@ -1,0 +1,20 @@
+import Semantics.Stlc.Syntax
+
+namespace Term
+namespace Natural
+
+inductive Value: Term → Prop where
+  | abs₁: Value (abs _ _ _)
+  | true₁: Value true
+  | false₁: Value false
+
+def subst (x: String) (s: Term) (t: Term): Term :=
+  match t with
+  | var y => bif x = y then s else t
+  | abs y T t₁ => bif x = y then t else abs y T (subst x s t₁)
+  | app t₁ t₂ => app (subst x s t₁) (subst x s t₂)
+  | cond t₁ t₂ t₃ => cond (subst x s t₁) (subst x s t₂) (subst x s t₃)
+  | otherwise => otherwise
+
+end Natural
+end Term
