Semantics/Stlc/Syntax.lean
@@ -1,0 +1,43 @@
+inductive Ty where
+  | Bool
+  | Arrow: Ty → Ty → Ty
+
+inductive Term where
+  | var: String → Term
+  | app: Term → Term → Term
+  | abs: String → Ty → Term → Term
+  | true
+  | false
+  | cond: Term → Term → Term → Term
+
+-- Syntax of the language
+declare_syntax_cat stlc
+
+syntax "(" stlc ")" : stlc
+syntax ident: stlc
+-- stmt
+syntax "λ" ident ":" stlc "↦" stlc : stlc
+syntax "if " stlc " then " stlc " else " stlc : stlc
+syntax stlc " → " stlc : stlc
+syntax stlc stlc : stlc
+-- meta
+syntax "⦃" stlc "⦄" : term
+
+macro_rules
+  -- keywords
+  | `(⦃true⦄)   => `(Term.true)
+  | `(⦃false⦄)  => `(Term.false)
+  | `(⦃Bool⦄)   => `(Ty.Bool)
+  | `(⦃$x → $y⦄) => `(Ty.Arrow ⦃$x⦄ ⦃$y⦄)
+  -- general
+  | `(⦃($x)⦄) => `(⦃$x⦄)
+  | `(⦃$x:ident⦄) => `(Term.var $(Lean.quote (toString x.getId)))
+  -- stlc
+  | `(⦃λ $x : $t ↦ $e⦄) => `(Term.abs $(Lean.quote (toString x.getId)) ⦃$t⦄ ⦃$e⦄)
+  | `(⦃$x $y⦄) => `(Term.app ⦃$x⦄ ⦃$y⦄)
+  | `(⦃if $b then $x else $y⦄) => `(Term.cond ⦃$b⦄ ⦃$x⦄ ⦃$y⦄)
+
+
+#check ⦃(λx:Bool↦x) true⦄
+#check ⦃(λx:Bool↦if x then false else true) true⦄
+#check ⦃λf:Bool→Bool↦f (f true)⦄
